concurrency/scache/cache/Cache_Refines_SimpleCache.i.dfy
@@ -1,6 +1,7 @@
 include "SimpleCacheSM.i.dfy"
 include "CacheSM.i.dfy"
 include "../Constants.i.dfy"
+include "CacheInv.i.dfy"
 
 module DiskSSM_Refines_SimpleCachine
   refines Refinement(CrashAsyncIfc(CacheIfc),
@@ -8,88 +9,155 @@ module DiskSSM_Refines_SimpleCachine
         SimpleCacheStateMachine)
 {
   import opened Constants
+  import opened NativeTypes
   import opened RequestIds
+  import opened CacheStatusType
   import opened Options
   import opened CacheSSM
   import CacheIfc
   import DiskIfc
+  import AsyncDisk
+  import opened CacheInv
 
-  predicate IsReading(machine: CacheSSM.M, addr: nat)
+  predicate Inv(s: A.Variables)
   {
-    && machine.M?
-    && addr in machine.disk_idx_to_cache_idx
-    && machine.disk_idx_to_cache_idx[addr].Some?
-    && machine.disk_idx_to_cache_idx[addr].value in machine.entries
-    && machine.entries[machine.disk_idx_to_cache_idx[addr].value].Reading?
-  }
-
-  predicate IsWriting(machine: CacheSSM.M, addr: nat)
-  {
-    && machine.M?
-    && addr in machine.disk_idx_to_cache_idx
-    && machine.disk_idx_to_cache_idx[addr].Some?
-    && machine.disk_idx_to_cache_idx[addr].value in machine.statuses
-    && machine.statuses[machine.disk_idx_to_cache_idx[addr].value].Writeback?
-  }
-
-  predicate InverseMapConsistent(machine: CacheSSM.M, i: nat)
-  {
-    && machine.M?
-    && i in machine.disk_idx_to_cache_idx ==>
-      && machine.disk_idx_to_cache_idx[i].Some? ==>
-        && machine.disk_idx_to_cache_idx[i].value in machine.entries
-        && (machine.entries[machine.disk_idx_to_cache_idx[i].value].Reading?
-          || machine.entries[machine.disk_idx_to_cache_idx[i].value].Entry?)
-        && machine.entries[machine.disk_idx_to_cache_idx[i].value].disk_idx == i
-  }
-
-  predicate Inv(s: A.Variables) {
-    && s.machine.M?
-    && (forall i :: i in s.machine.statuses <==>
-        (i in s.machine.entries && s.machine.entries[i].Entry?))
-    && (forall i | i in s.machine.entries ::
-        (s.machine.entries[i].Entry? || s.machine.entries[i].Reading?) ==>
-            s.machine.entries[i].disk_idx in s.machine.disk_idx_to_cache_idx &&
-            s.machine.disk_idx_to_cache_idx[s.machine.entries[i].disk_idx] == Some(i))
-
-    && (forall i :: InverseMapConsistent(s.machine, i))
-
-    && s.machine.read_reqs !! s.machine.read_resps.Keys
-    && (forall rid1, rid2 | rid1 in s.disk.reqReads && rid2 in s.disk.respReads ::
-          s.disk.reqReads[rid1].addr != s.disk.respReads[rid2].addr)
-    && (forall rid1 | rid1 in s.disk.reqReads :: s.disk.reqReads[rid1].addr !in s.machine.read_reqs)
-    && (forall rid1 | rid1 in s.disk.reqReads :: s.disk.reqReads[rid1].addr !in s.machine.read_resps)
-    && (forall rid2 | rid2 in s.disk.respReads :: s.disk.respReads[rid2].addr !in s.machine.read_reqs)
-    && (forall rid2 | rid2 in s.disk.respReads :: s.disk.respReads[rid2].addr !in s.machine.read_resps)
-    && (forall rid1 | rid1 in s.disk.reqReads :: IsReading(s.machine, s.disk.reqReads[rid1].addr))
-    && (forall rid2 | rid2 in s.disk.respReads :: IsReading(s.machine, s.disk.respReads[rid2].addr))
-    && (forall addr | addr in s.machine.read_reqs :: IsReading(s.machine, addr))
-    && (forall addr | addr in s.machine.read_resps :: IsReading(s.machine, addr))
-
-    && s.machine.write_reqs.Keys !! s.machine.write_resps
-    && (forall rid1, rid2 | rid1 in s.disk.reqWrites && rid2 in s.disk.respWrites ::
-          s.disk.reqWrites[rid1].addr != s.disk.respWrites[rid2].addr)
-    && (forall rid1 | rid1 in s.disk.reqWrites :: s.disk.reqWrites[rid1].addr !in s.machine.write_reqs)
-    && (forall rid1 | rid1 in s.disk.reqWrites :: s.disk.reqWrites[rid1].addr !in s.machine.write_resps)
-    && (forall rid2 | rid2 in s.disk.respWrites :: s.disk.respWrites[rid2].addr !in s.machine.write_reqs)
-    && (forall rid2 | rid2 in s.disk.respWrites :: s.disk.respWrites[rid2].addr !in s.machine.write_resps)
-    && (forall rid1 | rid1 in s.disk.reqWrites :: IsWriting(s.machine, s.disk.reqWrites[rid1].addr))
-    && (forall rid2 | rid2 in s.disk.respWrites :: IsWriting(s.machine, s.disk.respWrites[rid2].addr))
-    && (forall addr | addr in s.machine.write_reqs :: IsWriting(s.machine, addr))
-    && (forall addr | addr in s.machine.write_resps :: IsWriting(s.machine, addr))
+    CacheInv.Inv(s)
   }
 
   lemma InitImpliesInv(s: A.Variables)
   //requires A.Init(s)
   ensures Inv(s)
   {
+    CacheInv.InitImpliesInv(s);
   }
 
-  lemma Start_PreservesInv(s: A.Variables, s': A.Variables, rid: RequestId, input: CacheIfc.Input)
-  requires Inv(s)
-  requires A.NewTicket(s, s', rid, input)
+  lemma NextPreservesInv(s: A.Variables, s': A.Variables, op: ifc.Op)
+  //requires Inv(s)
+  //requires A.Next(s, s', op)
   ensures Inv(s')
   {
+    CacheInv.NextPreservesInv(s, s', op);
+  }
+
+  function IEntry(d: nat, entries: map<nat, Entry>, statuses: map<nat, Status>) : B.Entry
+  requires d in entries && entries[d].Entry? ==> d in statuses
+  {
+    if d in entries then
+      match entries[d] {
+        case Empty => B.Empty
+        case Reading(disk_idx) => B.Reading(disk_idx)
+        case Entry(disk_idx, data) =>
+          match statuses[d] {
+            case Clean => B.Clean(disk_idx, data)
+            case Dirty => B.Dirty(disk_idx, data)
+            case Writeback => B.Writeback(disk_idx, data)
+          }
+      }
+    else B.Empty
+  }
+
+  function IEntries(entries: map<nat, Entry>, statuses: map<nat, Status>) : imap<nat, B.Entry>
+  requires forall d :: d in entries && entries[d].Entry? ==> d in statuses
+  {
+    imap d | B.True(d) :: IEntry(d, entries, statuses)
+  }
+
+  function easy_union<K(!new),V>(m1: map<K, V>, m2: map<K, V>) : map<K, V> {
+    map k | k in m1.Keys + m2.Keys ::
+        if k in m1 then m1[k] else m2[k]
+  }
+
+  function {:opaque} map_of_write_reqs(m: map<RequestId, DiskIfc.ReqWrite>) : map<nat, seq<byte>>
+  requires forall rid1, rid2 | rid1 in m && rid2 in m && rid1 != rid2 :: m[rid1].addr != m[rid2].addr
+  {
+    map rid | rid in m :: m[rid].addr := m[rid].data
+  }
+
+  function {:opaque} map_of_read_resps(m: map<RequestId, DiskIfc.RespRead>) : map<nat, seq<byte>>
+  requires forall rid1, rid2 | rid1 in m && rid2 in m && rid1 != rid2 :: m[rid1].addr != m[rid2].addr
+  {
+    map rid | rid in m :: m[rid].addr := m[rid].data
+  }
+
+  function set_of_read_reqs(m: map<RequestId, DiskIfc.ReqRead>) : set<nat> {
+    set rid | rid in m :: m[rid].addr
+  }
+
+  function set_of_write_resps(m: map<RequestId, DiskIfc.RespWrite>) : set<nat> {
+    set rid | rid in m :: m[rid].addr
+  }
+
+  function IWriteReqs(mr: map<nat, DiskIfc.Block>, dr: map<RequestId, DiskIfc.ReqWrite>)
+      : map<nat, seq<byte>>
+  requires forall rid1, rid2 | rid1 in dr && rid2 in dr && rid1 != rid2 :: dr[rid1].addr != dr[rid2].addr
+  {
+    easy_union(mr, map_of_write_reqs(dr))
+  }
+
+  function IWriteResps(mr: set<nat>, dr: map<RequestId, DiskIfc.RespWrite>)
+      : set<nat>
+  {
+    mr + set_of_write_resps(dr)
+  }
+
+  function IReadReqs(mr: set<nat>, dr: map<RequestId, DiskIfc.ReqRead>)
+      : set<nat>
+  {
+    mr + set_of_read_reqs(dr)
+  }
+
+  function IReadResps(mr: map<nat, DiskIfc.Block>, dr: map<RequestId, DiskIfc.RespRead>)
+      : map<nat, seq<byte>>
+  requires forall rid1, rid2 | rid1 in dr && rid2 in dr && rid1 != rid2 :: dr[rid1].addr != dr[rid2].addr
+  {
+    easy_union(mr, map_of_read_resps(dr))
+  }
+
+  function IDisk(contents: map<nat, DiskIfc.Block>) : imap<nat, seq<byte>> {
+    imap addr | addr in contents :: contents[addr]
+  }
+
+  function I(s: A.Variables) : B.Variables
+  //requires Inv(s)
+  {
+    B.Variables(
+      IEntries(s.machine.entries, s.machine.statuses),
+      IWriteReqs(s.machine.write_reqs, s.disk.reqWrites),
+      IWriteResps(s.machine.write_resps, s.disk.respWrites),
+      IReadReqs(s.machine.read_reqs, s.disk.reqReads),
+      IReadResps(s.machine.read_resps, s.disk.respReads),
+      s.machine.tickets,
+      s.machine.stubs,
+      IDisk(s.disk.contents),
+      s.machine.sync_reqs
+    )
+  }
+
+  lemma InitRefinesInit(s: A.Variables)
+  //requires A.Init(s)
+  //requires Inv(s)
+  ensures B.Init(I(s))
+  {
+    assert I(s).write_reqs == map[] by {
+      reveal_map_of_write_reqs();
+    }
+    assert I(s).read_resps == map[] by {
+      reveal_map_of_read_resps();
+    }
+    assert I(s).entries == (imap k | B.True(k) :: B.Empty) by {
+      forall k | B.True(k)
+      ensures I(s).entries[k] == B.Empty
+      { }
+    }
+  }
+
+  lemma Start_Refines(s: A.Variables, s': A.Variables, rid: RequestId, input: CacheIfc.Input)
+  requires Inv(s)
+  requires A.NewTicket(s, s', rid, input)
+  requires Inv(s')
+  ensures B.Next(I(s), I(s'), ifc.Start(rid, input))
+  {
+    assume false;
     assert s'.machine.entries == s.machine.entries;
     assert s'.machine.statuses == s.machine.statuses;
     assert s'.machine.read_reqs == s.machine.read_reqs;
@@ -102,11 +170,13 @@ module DiskSSM_Refines_SimpleCachine
     assert forall i :: IsWriting(s.machine, i) ==> IsWriting(s'.machine, i);
   }
 
-  lemma End_PreservesInv(s: A.Variables, s': A.Variables, rid: RequestId, output: CacheIfc.Output)
+  lemma End_Refines(s: A.Variables, s': A.Variables, rid: RequestId, output: CacheIfc.Output)
   requires Inv(s)
   requires A.ConsumeStub(s, s', rid, output)
-  ensures Inv(s')
+  requires Inv(s')
+  ensures B.Next(I(s), I(s'), ifc.End(rid, output))
   {
+    assume false;
     assert s'.machine.entries == s.machine.entries;
     assert s'.machine.statuses == s.machine.statuses;
 
@@ -115,237 +185,653 @@ module DiskSSM_Refines_SimpleCachine
     assert forall i :: IsWriting(s.machine, i) ==> IsWriting(s'.machine, i);
   }
 
-  lemma StartRead_PreservesInv(s: A.Variables, s': A.Variables, cache_idx: nat, disk_idx: nat)
+  lemma StartRead_Refines(s: A.Variables, s': A.Variables, cache_idx: nat, disk_idx: nat)
   requires Inv(s)
   requires CacheSSM.StartRead(s.machine, s'.machine, cache_idx, disk_idx)
   requires s'.disk == s.disk
-  ensures Inv(s')
+  requires Inv(s')
+  ensures B.Next(I(s), I(s'), ifc.InternalOp)
+  {
+    assert B.StartRead(I(s), I(s'), ifc.InternalOp,
+          cache_idx, disk_idx);
+    assert B.NextStep(I(s), I(s'), ifc.InternalOp,
+          B.StartRead_Step(cache_idx, disk_idx));
+  }
 
-  lemma FinishRead_PreservesInv(s: A.Variables, s': A.Variables, cache_idx: nat, disk_idx: nat)
+  lemma FinishRead_Refines(s: A.Variables, s': A.Variables, cache_idx: nat, disk_idx: nat)
   requires Inv(s)
   requires CacheSSM.FinishRead(s.machine, s'.machine, cache_idx, disk_idx)
   requires s'.disk == s.disk
-  ensures Inv(s')
+  requires Inv(s')
+  ensures B.Next(I(s), I(s'), ifc.InternalOp)
+  {
+    assert disk_idx !in map_of_read_resps(s.disk.respReads) by {
+      reveal_map_of_read_resps();
+    }
+    assert B.FinishRead(I(s), I(s'), ifc.InternalOp,
+          cache_idx, disk_idx);
+    assert B.NextStep(I(s), I(s'), ifc.InternalOp,
+          B.FinishRead_Step(cache_idx, disk_idx));
+  }
 
-  lemma StartWriteback_PreservesInv(s: A.Variables, s': A.Variables, cache_idx: nat)
+  lemma StartWriteback_Refines(s: A.Variables, s': A.Variables, cache_idx: nat)
   requires Inv(s)
   requires CacheSSM.StartWriteback(s.machine, s'.machine, cache_idx)
   requires s'.disk == s.disk
-  ensures Inv(s')
+  requires Inv(s')
+  ensures B.Next(I(s), I(s'), ifc.InternalOp)
+  {
+    var disk_idx := s.machine.entries[cache_idx].disk_idx;
+    assert B.StartWriteback(I(s), I(s'), ifc.InternalOp,
+          cache_idx, disk_idx);
+    assert B.NextStep(I(s), I(s'), ifc.InternalOp,
+          B.StartWriteback_Step(cache_idx, disk_idx));
+  }
 
-  lemma FinishWriteback_PreservesInv(s: A.Variables, s': A.Variables, cache_idx: nat)
+  lemma FinishWriteback_Refines(s: A.Variables, s': A.Variables, cache_idx: nat)
   requires Inv(s)
   requires CacheSSM.FinishWriteback(s.machine, s'.machine, cache_idx)
   requires s'.disk == s.disk
-  ensures Inv(s')
+  requires Inv(s')
+  ensures B.Next(I(s), I(s'), ifc.InternalOp)
+  {
+    var disk_idx := s.machine.entries[cache_idx].disk_idx;
+    assert B.FinishWriteback(I(s), I(s'), ifc.InternalOp,
+          cache_idx, disk_idx);
+    assert B.NextStep(I(s), I(s'), ifc.InternalOp,
+          B.FinishWriteback_Step(cache_idx, disk_idx));
+  }
 
-  lemma Evict_PreservesInv(s: A.Variables, s': A.Variables, cache_idx: nat, disk_idx: nat, data: DiskIfc.Block, cache_idx2_opt: Option<nat>)
+  lemma Evict_Refines(s: A.Variables, s': A.Variables, cache_idx: nat)
   requires Inv(s)
-  requires CacheSSM.Evict(s.machine, s'.machine, cache_idx, disk_idx, data, cache_idx2_opt)
+  requires CacheSSM.Evict(s.machine, s'.machine, cache_idx)
   requires s'.disk == s.disk
-  ensures Inv(s')
+  requires Inv(s')
+  ensures B.Next(I(s), I(s'), ifc.InternalOp)
+  {
+    assert B.Evict(I(s), I(s'), ifc.InternalOp,
+          cache_idx);
+    assert B.NextStep(I(s), I(s'), ifc.InternalOp,
+          B.Evict_Step(cache_idx));
+  }
 
-  lemma ObserveCleanForSync_PreservesInv(s: A.Variables, s': A.Variables, cache_idx: nat, disk_idx: nat, data: DiskIfc.Block, rid: RequestId, se: set<nat>)
+  lemma ObserveCleanForSync_Refines(s: A.Variables, s': A.Variables, cache_idx: nat, rid: RequestId)
   requires Inv(s)
-  requires CacheSSM.ObserveCleanForSync(s.machine, s'.machine, cache_idx, disk_idx, data, rid, se)
+  requires CacheSSM.ObserveCleanForSync(s.machine, s'.machine, cache_idx, rid)
   requires s'.disk == s.disk
-  ensures Inv(s')
+  requires Inv(s')
+  ensures B.Next(I(s), I(s'), ifc.InternalOp)
+  {
+    assert B.ObserveCleanForSync(I(s), I(s'), ifc.InternalOp,
+          rid, cache_idx);
+    assert B.NextStep(I(s), I(s'), ifc.InternalOp,
+          B.ObserveCleanForSync_Step(rid, cache_idx));
+  }
 
-  lemma ApplyRead_PreservesInv(s: A.Variables, s': A.Variables, cache_idx: nat, disk_idx: nat, data: DiskIfc.Block, rid: RequestId)
+  lemma ApplyRead_Refines(s: A.Variables, s': A.Variables, cache_idx: nat, rid: RequestId)
   requires Inv(s)
-  requires CacheSSM.ApplyRead(s.machine, s'.machine, cache_idx, disk_idx, data, rid)
+  requires CacheSSM.ApplyRead(s.machine, s'.machine, cache_idx, rid)
   requires s'.disk == s.disk
-  ensures Inv(s')
+  requires Inv(s')
+  ensures B.Next(I(s), I(s'), ifc.InternalOp)
+  {
+    assert B.ApplyRead(I(s), I(s'), ifc.InternalOp,
+          rid, cache_idx);
+    assert B.NextStep(I(s), I(s'), ifc.InternalOp,
+          B.ApplyRead_Step(rid, cache_idx));
+  }
 
-  lemma ApplyWrite_PreservesInv(s: A.Variables, s': A.Variables, cache_idx: nat, disk_idx: nat, data: DiskIfc.Block, new_data: DiskIfc.Block, rid: RequestId)
+  lemma ApplyWrite_Refines(s: A.Variables, s': A.Variables, cache_idx: nat, rid: RequestId)
   requires Inv(s)
-  requires CacheSSM.ApplyWrite(s.machine, s'.machine, cache_idx, disk_idx, data, new_data, rid)
+  requires CacheSSM.ApplyWrite(s.machine, s'.machine, cache_idx, rid)
   requires s'.disk == s.disk
-  ensures Inv(s')
+  requires Inv(s')
+  ensures B.Next(I(s), I(s'), ifc.InternalOp)
+  {
+    assert B.ApplyWrite(I(s), I(s'), ifc.InternalOp,
+          rid, cache_idx);
+    assert B.NextStep(I(s), I(s'), ifc.InternalOp,
+          B.ApplyWrite_Step(rid, cache_idx));
+  }
 
-  lemma MarkDirty_PreservesInv(s: A.Variables, s': A.Variables, cache_idx: nat)
+  lemma MarkDirty_Refines(s: A.Variables, s': A.Variables, cache_idx: nat)
   requires Inv(s)
   requires CacheSSM.MarkDirty(s.machine, s'.machine, cache_idx)
   requires s'.disk == s.disk
-  ensures Inv(s')
-
-  lemma StartRead_Monotonic(s: A.Variables, s': A.Variables, rest: CacheSSM.M,
-      cache_idx: nat, disk_idx: nat)
-  requires Inv(A.Variables(s.disk, CacheSSM.dot(s.machine, rest)))
-  requires CacheSSM.StartRead(s.machine, s'.machine, cache_idx, disk_idx)
-  ensures CacheSSM.Internal(CacheSSM.dot(s.machine, rest), CacheSSM.dot(s'.machine, rest))
+  requires Inv(s')
+  ensures B.Next(I(s), I(s'), ifc.InternalOp)
   {
-    /*assert disk_idx in s.machine.read_reqs ==> IsReading(s.machine, disk_idx);
-    var f := CacheSSM.dot(s.machine, rest);
-    var f' := CacheSSM.dot(s'.machine, rest);
-    assert f'.M?;
-    assert (f'.entries == f.entries[cache_idx := CacheSSM.Reading(disk_idx)]);
-    assert (f'.disk_idx_to_cache_idx == f.disk_idx_to_cache_idx[disk_idx := Some(cache_idx)]);
-    assert (f'.read_reqs == f.read_reqs + {disk_idx});*/
-    assert CacheSSM.StartRead(CacheSSM.dot(s.machine, rest), CacheSSM.dot(s'.machine, rest), cache_idx, disk_idx);
-    assert CacheSSM.InternalStep(CacheSSM.dot(s.machine, rest), CacheSSM.dot(s'.machine, rest), CacheSSM.StartReadStep(cache_idx, disk_idx));
+    assume false;
+    //assert B.MarkDirty(I(s), I(s'), ifc.InternalOp, cache_idx);
+    //assert B.NextStep(I(s), I(s'), ifc.InternalOp, B.MarkDirty_Step(cache_idx));
   }
 
-  lemma FinishRead_Monotonic(s: A.Variables, s': A.Variables, rest: CacheSSM.M,
-      cache_idx: nat, disk_idx: nat)
-  requires Inv(A.Variables(s.disk, CacheSSM.dot(s.machine, rest)))
-  requires CacheSSM.FinishRead(s.machine, s'.machine, cache_idx, disk_idx)
-  ensures CacheSSM.Internal(CacheSSM.dot(s.machine, rest), CacheSSM.dot(s'.machine, rest))
-  {
-    assert CacheSSM.InternalStep(CacheSSM.dot(s.machine, rest), CacheSSM.dot(s'.machine, rest), CacheSSM.FinishReadStep(cache_idx, disk_idx));
-  }
-
-  lemma StartWriteback_Monotonic(s: A.Variables, s': A.Variables, rest: CacheSSM.M,
-      cache_idx: nat)
-  requires Inv(A.Variables(s.disk, CacheSSM.dot(s.machine, rest)))
-  requires CacheSSM.StartWriteback(s.machine, s'.machine, cache_idx)
-  ensures CacheSSM.Internal(CacheSSM.dot(s.machine, rest), CacheSSM.dot(s'.machine, rest))
-  {
-    var disk_idx := s.machine.entries[cache_idx].disk_idx;
-    var f := CacheSSM.dot(s.machine, rest);
-    assert disk_idx in f.write_reqs ==> IsWriting(f, disk_idx);
-    assert CacheSSM.StartWriteback(CacheSSM.dot(s.machine, rest), CacheSSM.dot(s'.machine, rest), cache_idx);
-    assert CacheSSM.InternalStep(CacheSSM.dot(s.machine, rest), CacheSSM.dot(s'.machine, rest), CacheSSM.StartWritebackStep(cache_idx));
-  }
-
-  lemma FinishWriteback_Monotonic(s: A.Variables, s': A.Variables, rest: CacheSSM.M,
-      cache_idx: nat)
-  requires Inv(A.Variables(s.disk, CacheSSM.dot(s.machine, rest)))
-  requires CacheSSM.FinishWriteback(s.machine, s'.machine, cache_idx)
-  ensures CacheSSM.Internal(CacheSSM.dot(s.machine, rest), CacheSSM.dot(s'.machine, rest))
-  {
-    assert CacheSSM.InternalStep(CacheSSM.dot(s.machine, rest), CacheSSM.dot(s'.machine, rest), CacheSSM.FinishWritebackStep(cache_idx));
-  }
-
-  lemma InternalMonotonic(s: A.Variables, s': A.Variables, rest: CacheSSM.M)
-  requires Inv(A.Variables(s.disk, CacheSSM.dot(s.machine, rest)))
-  requires CacheSSM.Internal(s.machine, s'.machine)
-  ensures CacheSSM.Internal(CacheSSM.dot(s.machine, rest), CacheSSM.dot(s'.machine, rest))
-  {
-    var step :| CacheSSM.InternalStep(s.machine, s'.machine, step);
-    match step {
-      case StartReadStep(cache_idx, disk_idx) => {
-        StartRead_Monotonic(s, s', rest, cache_idx, disk_idx);
-      }
-
-      case FinishReadStep(cache_idx, disk_idx) => {
-        assume false;
-        assert CacheSSM.InternalStep(CacheSSM.dot(s.machine, rest), CacheSSM.dot(s'.machine, rest), step);
-      }
-
-      case StartWritebackStep(cache_idx) => {
-        assume false;
-        assert CacheSSM.Internal(CacheSSM.dot(s.machine, rest), CacheSSM.dot(s'.machine, rest));
-      }
-
-      case FinishWritebackStep(cache_idx) => {
-        assume false;
-        assert CacheSSM.Internal(CacheSSM.dot(s.machine, rest), CacheSSM.dot(s'.machine, rest));
-      }
-
-      case EvictStep(cache_idx, disk_idx, data, cache_idx2_opt) => {
-        assume false;
-        assert CacheSSM.Internal(CacheSSM.dot(s.machine, rest), CacheSSM.dot(s'.machine, rest));
-      }
-
-      case ObserveCleanForSyncStep(cache_idx, disk_idx, data, rid, se) => {
-        assume false;
-        assert CacheSSM.Internal(CacheSSM.dot(s.machine, rest), CacheSSM.dot(s'.machine, rest));
-      }
-
-      case ApplyReadStep(cache_idx, disk_idx, data, rid) => {
-        assume false;
-        assert CacheSSM.Internal(CacheSSM.dot(s.machine, rest), CacheSSM.dot(s'.machine, rest));
-      }
-
-      case ApplyWriteStep(cache_idx, disk_idx, data, new_data, rid) => {
-        assume false;
-        assert CacheSSM.Internal(CacheSSM.dot(s.machine, rest), CacheSSM.dot(s'.machine, rest));
-      }
-
-      case MarkDirtyStep(cache_idx) => {
-        assume false;
-        assert CacheSSM.Internal(CacheSSM.dot(s.machine, rest), CacheSSM.dot(s'.machine, rest));
-      }
-    }
-  }
-
-/*
-  lemma Internal_PreservesInv(s: A.Variables, s': A.Variables)
+  lemma Machine_Internal_Refines(s: A.Variables, s': A.Variables)
   requires Inv(s)
-  requires A.Machine(s, s')
-  ensures Inv(s')
+  requires Internal(s.machine, s'.machine)
+  requires s.disk == s'.disk
+  requires Inv(s')
+  ensures B.Next(I(s), I(s'), ifc.InternalOp)
   {
     var step :| CacheSSM.InternalStep(s.machine, s'.machine, step);
     match step {
       case StartReadStep(cache_idx, disk_idx) =>
-        StartRead_PreservesInv(s, s', cache_idx, disk_idx);
+        StartRead_Refines(s, s', cache_idx, disk_idx);
 
       case FinishReadStep(cache_idx, disk_idx) => 
-        FinishRead_PreservesInv(s, s', cache_idx, disk_idx);
+        FinishRead_Refines(s, s', cache_idx, disk_idx);
 
-      case StartWritebackStep(cache_idx, disk_idx, data) =>
-        StartWriteback_PreservesInv(s, s', cache_idx, disk_idx, data);
+      case StartWritebackStep(cache_idx) =>
+        StartWriteback_Refines(s, s', cache_idx);
 
-      case FinishWritebackStep(cache_idx, disk_idx, data) =>
-        FinishWriteback_PreservesInv(s, s', cache_idx, disk_idx, data);
+      case FinishWritebackStep(cache_idx) =>
+        FinishWriteback_Refines(s, s', cache_idx);
 
-      case EvictStep(cache_idx, disk_idx, data, cache_idx2_opt) =>
-        Evict_PreservesInv(s, s', cache_idx, disk_idx, data, cache_idx2_opt);
+      case EvictStep(cache_idx) =>
+        Evict_Refines(s, s', cache_idx);
 
-      case ObserveCleanForSyncStep(cache_idx, disk_idx, data, rid, se) =>
-        ObserveCleanForSync_PreservesInv(s, s', cache_idx, disk_idx, data, rid, se);
+      case ObserveCleanForSyncStep(cache_idx, rid) =>
+        ObserveCleanForSync_Refines(s, s', cache_idx, rid);
 
-      case ApplyReadStep(cache_idx, disk_idx, data, rid) =>
-        ApplyRead_PreservesInv(s, s', cache_idx, disk_idx, data, rid);
+      case ApplyReadStep(cache_idx, rid) =>
+        ApplyRead_Refines(s, s', cache_idx, rid);
 
-      case ApplyWriteStep(cache_idx, disk_idx, data, new_data, rid) =>
-        ApplyWrite_PreservesInv(s, s', cache_idx, disk_idx, data, new_data, rid);
+      case ApplyWriteStep(cache_idx, rid) =>
+        ApplyWrite_Refines(s, s', cache_idx, rid);
 
       case MarkDirtyStep(cache_idx) =>
-        MarkDirty_PreservesInv(s, s', cache_idx);
-    }
-  }
-  */
-
-  lemma NextPreservesInv(s: A.Variables, s': A.Variables, op: ifc.Op)
-  //requires Inv(s)
-  //requires A.Next(s, s', op)
-  ensures Inv(s')
-  {
-    match op {
-      case Start(rid, input) => {
-        Start_PreservesInv(s, s', rid, input);
-      }
-      case End(rid, output) => {
-        End_PreservesInv(s, s', rid, output);
-      }
-      case CrashOp => {
-        InitImpliesInv(s');
-      }
-      case InternalOp => {
-        assume false;
-        //Internal_PreservesInv(s, s');
-      }
+        MarkDirty_Refines(s, s', cache_idx);
     }
   }
 
-  function I(s: A.Variables) : B.Variables
-  //requires Inv(s)
-
-  lemma InitRefinesInit(s: A.Variables)
-  //requires A.Init(s)
-  //requires Inv(s)
-  ensures B.Init(I(s))
+  lemma ProcessRead_Refines(s: A.Variables, s': A.Variables, id: RequestId)
+  requires Inv(s)
+  requires AsyncDisk.ProcessRead(s.disk, s'.disk, id)
+  requires s.machine == s'.machine
+  requires Inv(s')
+  ensures B.Next(I(s), I(s'), ifc.InternalOp)
   {
+    var disk_idx := s.disk.reqReads[id].addr;
+
+    assert IReadResps(s'.machine.read_resps, s'.disk.respReads)
+        == IReadResps(s.machine.read_resps, s.disk.respReads)[disk_idx := I(s).disk[disk_idx]]
+    by {
+      assert map_of_read_resps(s'.disk.respReads)
+          == map_of_read_resps(s.disk.respReads)[disk_idx := s.disk.contents[disk_idx]]
+      by {
+        var x := map_of_read_resps(s.disk.respReads);
+        var y := map_of_read_resps(s'.disk.respReads);
+        assert disk_idx in y && y[disk_idx] == s.disk.contents[disk_idx] by {
+          assert s'.disk.respReads[id].addr == disk_idx;
+          assert s'.disk.respReads[id].data == s.disk.contents[disk_idx];
+          reveal_map_of_read_resps();
+        }
+        forall k | k in x && k != disk_idx
+        ensures k in y && x[k] == y[k]
+        {
+          /*
+          assert exists rid :: rid in s.disk.respReads
+              && s.disk.respReads[rid].addr == k by { reveal_map_of_read_resps(); }
+          var rid :| rid in s.disk.respReads
+              && s.disk.respReads[rid].addr == k;
+          assert rid != id;
+          assert rid in s'.disk.respReads
+              && s'.disk.respReads[rid].addr == k;
+          */
+          reveal_map_of_read_resps();
+        }
+        forall k | k in y && k != disk_idx
+        ensures k in x
+        {
+          reveal_map_of_read_resps();
+        }
+      }
+    }
+
+    assert IReadReqs(s'.machine.read_reqs, s'.disk.reqReads)
+        == IReadReqs(s.machine.read_reqs, s.disk.reqReads) - {disk_idx}
+    by {
+      //assert disk_idx !in s'.machine.read_reqs;
+      //assert disk_idx !in set_of_read_reqs(s'.disk.reqReads);
+      //forall k | k != disk_idx && k in set_of_read_reqs(s'.disk.reqReads)
+      //ensures k in set_of_read_reqs(s.disk.reqReads)
+      //{
+      //}
+      forall k | k != disk_idx && k in set_of_read_reqs(s.disk.reqReads)
+      ensures k in set_of_read_reqs(s'.disk.reqReads)
+      {
+        var y :| y in s.disk.reqReads && s.disk.reqReads[y].addr == k;
+        assert s'.disk.reqReads[y].addr == k;
+      }
+      //assert set_of_read_reqs(s'.disk.reqReads)
+      //      == set_of_read_reqs(s.disk.reqReads) - {disk_idx};
+    }
+
+    assert I(s).entries == I(s').entries;
+    assert I(s).write_reqs == I(s').write_reqs;
+    assert I(s).write_resps == I(s').write_resps;
+    assert I(s).tickets == I(s').tickets;
+    assert I(s).stubs == I(s').stubs;
+    assert I(s).disk == I(s').disk;
+    assert I(s).sync_reqs == I(s').sync_reqs;
+
+    assert B.ProcessRead(I(s), I(s'), ifc.InternalOp, disk_idx);
+    assert B.NextStep(I(s), I(s'), ifc.InternalOp,
+          B.ProcessRead_Step(disk_idx));
+  }
+
+  lemma ProcessWrite_Refines(s: A.Variables, s': A.Variables, id: RequestId)
+  requires Inv(s)
+  requires AsyncDisk.ProcessWrite(s.disk, s'.disk, id)
+  requires s.machine == s'.machine
+  requires Inv(s')
+  ensures B.Next(I(s), I(s'), ifc.InternalOp)
+  {
+    var disk_idx := s.disk.reqWrites[id].addr;
+
+    assert IWriteResps(s'.machine.write_resps, s'.disk.respWrites)
+        == IWriteResps(s.machine.write_resps, s.disk.respWrites) + {disk_idx}
+    by {
+      assert set_of_write_resps(s'.disk.respWrites)
+          == set_of_write_resps(s.disk.respWrites) + {disk_idx}
+      by {
+        var x := set_of_write_resps(s.disk.respWrites);
+        var y := set_of_write_resps(s'.disk.respWrites);
+        assert disk_idx in y by {
+          assert s'.disk.respWrites[id].addr == disk_idx;
+        }
+        forall k | k != disk_idx && k in x ensures k in y {
+          var rid :| rid in s.disk.respWrites && s.disk.respWrites[rid].addr == k;
+          assert rid in s'.disk.respWrites && s'.disk.respWrites[rid].addr == k;
+        }
+        forall k | k != disk_idx && k in y ensures k in x {
+        }
+      }
+    }
+
+    assert disk_idx in IWriteReqs(s.machine.write_reqs, s.disk.reqWrites)
+    by {
+      assert disk_idx in map_of_write_reqs(s.disk.reqWrites)
+      by {
+        reveal_map_of_write_reqs();
+      }
+    }
+
+    assert IWriteReqs(s'.machine.write_reqs, s'.disk.reqWrites)
+        == IWriteReqs(s.machine.write_reqs, s.disk.reqWrites) - {disk_idx}
+    by {
+      assert map_of_write_reqs(s'.disk.reqWrites)
+          == map_of_write_reqs(s.disk.reqWrites) - {disk_idx}
+      by {
+        var x := map_of_write_reqs(s.disk.reqWrites);
+        var y := map_of_write_reqs(s'.disk.reqWrites);
+        assert disk_idx !in y
+        by {
+          reveal_map_of_write_reqs();
+        }
+        forall k | k in x && k != disk_idx
+        ensures k in y && x[k] == y[k]
+        {
+          assert exists rid :: rid in s.disk.reqWrites && s.disk.reqWrites[rid].addr == k
+            by { reveal_map_of_write_reqs(); }
+          var rid :| rid in s.disk.reqWrites && s.disk.reqWrites[rid].addr == k;
+          assert rid != id;
+          assert rid in s'.disk.reqWrites && s'.disk.reqWrites[rid].addr == k;
+          reveal_map_of_write_reqs();
+        }
+        forall k | k in y && k != disk_idx
+        ensures k in x
+        {
+          reveal_map_of_write_reqs();
+        }
+      }
+    }
+
+    assert IWriteReqs(s.machine.write_reqs, s.disk.reqWrites)[disk_idx]
+      == s.disk.reqWrites[id].data
+    by {
+      reveal_map_of_write_reqs();
+    }
+
+    assert I(s').disk == I(s).disk[disk_idx := I(s).write_reqs[disk_idx]];
+
+    assert I(s).entries == I(s').entries;
+    assert I(s).read_reqs == I(s').read_reqs;
+    assert I(s).read_resps == I(s').read_resps;
+    assert I(s).tickets == I(s').tickets;
+    assert I(s).stubs == I(s').stubs;
+    assert I(s).sync_reqs == I(s').sync_reqs;
+
+    assert B.ProcessWrite(I(s), I(s'), ifc.InternalOp, disk_idx);
+    assert B.NextStep(I(s), I(s'), ifc.InternalOp,
+          B.ProcessWrite_Step(disk_idx));
+  }
+
+  lemma HavocConflictingWrites_Refines(s: A.Variables, s': A.Variables, id: RequestId, id':RequestId)
+  requires Inv(s)
+  requires AsyncDisk.HavocConflictingWrites(s.disk, s'.disk, id, id')
+  requires s.machine == s'.machine
+  requires Inv(s')
+  ensures B.Next(I(s), I(s'), ifc.InternalOp)
+  {
+    assert false; // premises are impossible
+  }
+
+  lemma HavocConflictingWriteRead_Refines(s: A.Variables, s': A.Variables, id: RequestId,id': RequestId)
+  requires Inv(s)
+  requires AsyncDisk.HavocConflictingWriteRead(s.disk, s'.disk, id, id')
+  requires s.machine == s'.machine
+  requires Inv(s')
+  ensures B.Next(I(s), I(s'), ifc.InternalOp)
+  {
+    assert false; // premises are impossible
+  }
+
+  lemma DiskInternal_Refines(s: A.Variables, s': A.Variables)
+  requires Inv(s)
+  requires A.DiskInternal(s, s')
+  requires Inv(s')
+  ensures B.Next(I(s), I(s'), ifc.InternalOp)
+  {
+    var step :| AsyncDisk.NextInternalStep(s.disk, s'.disk, step);
+    match step {
+      case ProcessReadStep(id) => ProcessRead_Refines(s, s', id);
+      case ProcessWriteStep(id) => ProcessWrite_Refines(s, s', id);
+      case HavocConflictingWritesStep(id, id') => HavocConflictingWrites_Refines(s, s', id, id');
+      case HavocConflictingWriteReadStep(id, id') => HavocConflictingWriteRead_Refines(s, s', id, id');
+    }
+  }
+
+  lemma Interaction_ReqWrite_Refines_helper(s: A.Variables, s': A.Variables, dop: DiskIfc.DiskOp)
+  requires Inv(s)
+  requires AsyncDisk.RecvWrite(s.disk, s'.disk, dop)
+  //requires s.machine == CacheSSM.dot(s'.machine, CacheSSM.DiskWriteReq(dop.reqWrite.addr, dop.reqWrite.data))
+
+  requires Inv(s')
+
+  requires s.machine == s'.machine.(
+    write_reqs := s'.machine.write_reqs[dop.reqWrite.addr := dop.reqWrite.data])
+
+  ensures B.Next(I(s), I(s'), ifc.InternalOp)
+  {
+    var disk_idx := dop.reqWrite.addr;
+    assert IWriteReqs(s'.machine.write_reqs, s'.disk.reqWrites)
+        == IWriteReqs(s.machine.write_reqs, s.disk.reqWrites)
+    by {
+      assert disk_idx in IWriteReqs(s.machine.write_reqs, s.disk.reqWrites);
+      assert disk_idx in IWriteReqs(s'.machine.write_reqs, s'.disk.reqWrites)
+          && IWriteReqs(s.machine.write_reqs, s.disk.reqWrites)[disk_idx]
+          == IWriteReqs(s'.machine.write_reqs, s'.disk.reqWrites)[disk_idx]
+      by {
+        assert s'.disk.reqWrites[dop.id].addr == disk_idx;
+        reveal_map_of_write_reqs();
+      }
+      var x := map_of_write_reqs(s.disk.reqWrites);
+      var y := map_of_write_reqs(s'.disk.reqWrites);
+      forall k | k != disk_idx && k in x
+      ensures k in y && y[k] == x[k]
+      {
+        reveal_map_of_write_reqs();
+      }
+      forall k | k != disk_idx && k in y
+      ensures k in x
+      {
+        reveal_map_of_write_reqs();
+      }
+    }
+    assert I(s) == I(s');
+    assert B.NextStep(I(s), I(s'), ifc.InternalOp, B.Stutter_Step);
+  }
+
+  lemma Interaction_RespWrite_Refines_helper(s: A.Variables, s': A.Variables, dop: DiskIfc.DiskOp)
+  requires Inv(s)
+  requires AsyncDisk.AckWrite(s.disk, s'.disk, dop)
+  //requires s'.machine == CacheSSM.dot(s.machine, CacheSSM.DiskWriteResp(dop.respWrite.addr))
+  requires s'.machine == s.machine.(
+    write_resps := s.machine.write_resps + {dop.respWrite.addr})
+  requires Inv(s')
+  ensures B.Next(I(s), I(s'), ifc.InternalOp)
+  {
+    var disk_idx := dop.respWrite.addr;
+    assert IWriteResps(s'.machine.write_resps, s'.disk.respWrites)
+        == IWriteResps(s.machine.write_resps, s.disk.respWrites)
+    by {
+      assert disk_idx in IWriteResps(s'.machine.write_resps, s'.disk.respWrites);
+      assert disk_idx in IWriteResps(s.machine.write_resps, s.disk.respWrites);
+      var x := set_of_write_resps(s.disk.respWrites);
+      var y := set_of_write_resps(s'.disk.respWrites);
+      forall k | k != disk_idx && k in x
+      ensures k in y
+      {
+        var id :| id in s.disk.respWrites && s.disk.respWrites[id].addr == k;
+        assert id != dop.id;
+        assert id in s'.disk.respWrites && s'.disk.respWrites[id].addr == k;
+      }
+      forall k | k != disk_idx && k in y
+      ensures k in x
+      {
+      }
+    }
+    assert I(s) == I(s');
+    assert B.NextStep(I(s), I(s'), ifc.InternalOp, B.Stutter_Step);
+  }
+
+  lemma Interaction_ReqRead_Refines_helper(s: A.Variables, s': A.Variables, dop: DiskIfc.DiskOp)
+  requires Inv(s)
+  requires AsyncDisk.RecvRead(s.disk, s'.disk, dop)
+  //requires s.machine == CacheSSM.dot(s'.machine, CacheSSM.DiskReadReq(dop.reqRead.addr))
+  requires Inv(s')
+  requires s.machine == s'.machine.(
+      read_reqs := s'.machine.read_reqs + {dop.reqRead.addr})
+  ensures B.Next(I(s), I(s'), ifc.InternalOp)
+  {
+    var disk_idx := dop.reqRead.addr;
+    assert IReadReqs(s'.machine.read_reqs, s'.disk.reqReads)
+        == IReadReqs(s.machine.read_reqs, s.disk.reqReads)
+    by {
+      assert disk_idx in IReadReqs(s'.machine.read_reqs, s'.disk.reqReads)
+      by {
+        assert s'.disk.reqReads[dop.id].addr == disk_idx;
+      }
+      assert disk_idx in IReadReqs(s.machine.read_reqs, s.disk.reqReads);
+      var x := set_of_read_reqs(s.disk.reqReads);
+      var y := set_of_read_reqs(s'.disk.reqReads);
+      forall k | k != disk_idx && k in x
+      ensures k in y
+      {
+        var id :| id in s.disk.reqReads && s.disk.reqReads[id].addr == k;
+        assert id != dop.id;
+        assert id in s'.disk.reqReads && s'.disk.reqReads[id].addr == k;
+      }
+      forall k | k != disk_idx && k in y
+      ensures k in x
+      {
+      }
+    }
+    assert I(s) == I(s');
+    assert B.NextStep(I(s), I(s'), ifc.InternalOp, B.Stutter_Step);
+  }
+
+  lemma Interaction_RespRead_Refines_helper(s: A.Variables, s': A.Variables, dop: DiskIfc.DiskOp)
+  requires Inv(s)
+  requires AsyncDisk.AckRead(s.disk, s'.disk, dop)
+  //requires s'.machine == CacheSSM.dot(s.machine, CacheSSM.DiskReadResp(dop.respRead.addr, dop.respRead.data))
+  requires Inv(s')
+  requires s'.machine == s.machine.(
+      read_resps := s.machine.read_resps[dop.respRead.addr := dop.respRead.data])
+  ensures B.Next(I(s), I(s'), ifc.InternalOp)
+  {
+    var disk_idx := dop.respRead.addr;
+    assert IReadResps(s'.machine.read_resps, s'.disk.respReads)
+        == IReadResps(s.machine.read_resps, s.disk.respReads)
+    by {
+      assert disk_idx in IReadResps(s'.machine.read_resps, s'.disk.respReads);
+      assert disk_idx in IReadResps(s.machine.read_resps, s.disk.respReads)
+          && IReadResps(s'.machine.read_resps, s'.disk.respReads)[disk_idx]
+          == IReadResps(s.machine.read_resps, s.disk.respReads)[disk_idx]
+      by {
+        assert s.disk.respReads[dop.id].addr == disk_idx;
+        reveal_map_of_read_resps();
+      }
+      var x := map_of_read_resps(s.disk.respReads);
+      var y := map_of_read_resps(s'.disk.respReads);
+      forall k | k != disk_idx && k in x
+      ensures k in y && y[k] == x[k]
+      {
+        assert exists rid :: rid in s.disk.respReads && s.disk.respReads[rid].addr == k by { reveal_map_of_read_resps(); }
+        var rid :| rid in s.disk.respReads && s.disk.respReads[rid].addr == k;
+        assert rid != dop.id;
+        assert s'.disk.respReads[rid].addr == k;
+        reveal_map_of_read_resps();
+      }
+      forall k | k != disk_idx && k in y
+      ensures k in x
+      {
+        reveal_map_of_read_resps();
+      }
+    }
+    assert I(s) == I(s');
+    assert B.NextStep(I(s), I(s'), ifc.InternalOp, B.Stutter_Step);
+  }
+
+  lemma Interaction_ReqWrite_Refines(s: A.Variables, s': A.Variables, dop: DiskIfc.DiskOp)
+  requires Inv(s)
+  requires AsyncDisk.RecvWrite(s.disk, s'.disk, dop)
+  requires s.machine == CacheSSM.dot(s'.machine, CacheSSM.DiskWriteReq(dop.reqWrite.addr, dop.reqWrite.data))
+  requires Inv(s')
+  ensures B.Next(I(s), I(s'), ifc.InternalOp)
+  {
+    assert s.machine.write_reqs ==
+      s'.machine.write_reqs[dop.reqWrite.addr := dop.reqWrite.data];
+    assert s.machine.disk_idx_to_cache_idx == s'.machine.disk_idx_to_cache_idx;
+    assert s.machine.entries == s'.machine.entries;
+    assert s.machine.statuses == s'.machine.statuses;
+    assert s.machine.read_reqs == s'.machine.read_reqs;
+    assert s.machine.read_resps == s'.machine.read_resps;
+    assert s.machine.write_resps == s'.machine.write_resps;
+    assert s.machine.tickets == s'.machine.tickets;
+    assert s.machine.stubs == s'.machine.stubs;
+    assert s.machine.sync_reqs == s'.machine.sync_reqs;
+    Interaction_ReqWrite_Refines_helper(s, s', dop);
+  }
+
+  lemma Interaction_RespWrite_Refines(s: A.Variables, s': A.Variables, dop: DiskIfc.DiskOp)
+  requires Inv(s)
+  requires AsyncDisk.AckWrite(s.disk, s'.disk, dop)
+  requires s'.machine == CacheSSM.dot(s.machine, CacheSSM.DiskWriteResp(dop.respWrite.addr))
+  requires Inv(s')
+  ensures B.Next(I(s), I(s'), ifc.InternalOp)
+  {
+    Interaction_RespWrite_Refines_helper(s, s', dop);
+  }
+
+  lemma Interaction_ReqRead_Refines(s: A.Variables, s': A.Variables, dop: DiskIfc.DiskOp)
+  requires Inv(s)
+  requires AsyncDisk.RecvRead(s.disk, s'.disk, dop)
+  requires s.machine == CacheSSM.dot(s'.machine, CacheSSM.DiskReadReq(dop.reqRead.addr))
+  requires Inv(s')
+  ensures B.Next(I(s), I(s'), ifc.InternalOp)
+  {
+    assert s.machine.read_reqs ==
+        s'.machine.read_reqs + {dop.reqRead.addr};
+    assert s.machine.disk_idx_to_cache_idx == s'.machine.disk_idx_to_cache_idx;
+    assert s.machine.entries == s'.machine.entries;
+    assert s.machine.statuses == s'.machine.statuses;
+    assert s.machine.write_reqs == s'.machine.write_reqs;
+    assert s.machine.read_resps == s'.machine.read_resps;
+    assert s.machine.write_resps == s'.machine.write_resps;
+    assert s.machine.tickets == s'.machine.tickets;
+    assert s.machine.stubs == s'.machine.stubs;
+    Interaction_ReqRead_Refines_helper(s, s', dop);
+  }
+
+  lemma Interaction_RespRead_Refines(s: A.Variables, s': A.Variables, dop: DiskIfc.DiskOp)
+  requires Inv(s)
+  requires AsyncDisk.AckRead(s.disk, s'.disk, dop)
+  requires s'.machine == CacheSSM.dot(s.machine, CacheSSM.DiskReadResp(dop.respRead.addr, dop.respRead.data))
+  requires Inv(s')
+  ensures B.Next(I(s), I(s'), ifc.InternalOp)
+  {
+    Interaction_RespRead_Refines_helper(s, s', dop);
+  }
+
+  lemma Interaction_Refines(s: A.Variables, s': A.Variables, dop: DiskIfc.DiskOp)
+  requires Inv(s)
+  requires A.Interaction(s, s', dop)
+  requires Inv(s')
+  ensures B.Next(I(s), I(s'), ifc.InternalOp)
+  {
+    match dop {
+      case ReqReadOp(id, reqRead) => {
+        Interaction_ReqRead_Refines(s, s', dop);
+      }
+      case ReqWriteOp(id, reqWrite) => {
+        Interaction_ReqWrite_Refines(s, s', dop);
+      }
+      case RespReadOp(id, respRead) => {
+        Interaction_RespRead_Refines(s, s', dop);
+      }
+      case RespWriteOp(id, respWrite) => {
+        Interaction_RespWrite_Refines(s, s', dop);
+      }
+    }
+  }
+
+  lemma Internal_Refines(s: A.Variables, s': A.Variables)
+  requires Inv(s)
+  requires A.Internal(s, s')
+  requires Inv(s')
+  ensures B.Next(I(s), I(s'), ifc.InternalOp)
+  {
+    var step :| A.InternalStep(s, s', step);
+    match step {
+      case MachineStep(shard, shard', rest) => {
+        InternalMonotonic(
+            A.Variables(s.disk, shard),
+            A.Variables(s.disk, shard'),
+            rest);
+        Machine_Internal_Refines(s, s');
+      }
+      case InteractionStep(dop) => {
+        Interaction_Refines(s, s', dop);
+      }
+      case DiskInternalStep => {
+        DiskInternal_Refines(s, s');
+      }
+    }
+  }
+
+  lemma Crash_Refines(s: A.Variables, s': A.Variables)
+  requires Inv(s)
+  requires A.Crash(s, s')
+  requires Inv(s')
+  ensures B.Next(I(s), I(s'), ifc.CrashOp)
+  {
+    InitImpliesInv(s');
+    InitRefinesInit(s');
+    assert B.Crash(I(s), I(s'), ifc.CrashOp);
+    assert B.NextStep(I(s), I(s'), ifc.CrashOp, B.Crash_Step);
   }
 
   lemma NextRefinesNext(s: A.Variables, s': A.Variables, op: ifc.Op)
   //requires Inv(s)
-  //requires Inv(s')
   //requires A.Next(s, s', op)
+  //requires Inv(s')
   ensures B.Next(I(s), I(s'), op)
   {
+    match op {
+      case Start(rid, input) => {
+        Start_Refines(s, s', rid, input);
+      }
+      case End(rid, output) => {
+        End_Refines(s, s', rid, output);
+      }
+      case CrashOp => {
+        Crash_Refines(s, s');
+      }
+      case InternalOp => {
+        Internal_Refines(s, s');
+      }
+    }
   }
-
 }
