concurrency/scache/cache/CacheInv.i.dfy
@@ -1,0 +1,621 @@
+include "SimpleCacheSM.i.dfy"
+include "CacheSM.i.dfy"
+include "../Constants.i.dfy"
+
+module CacheInv {
+  import ifc = CrashAsyncIfc(CacheIfc)
+  import A = AsyncDiskSystemStateMachine(CacheIfc, CacheSSM)
+
+  import opened Constants
+  import opened RequestIds
+  import opened Options
+  import opened CacheSSM
+  import CacheIfc
+  import DiskIfc
+  import AsyncDisk
+
+  predicate IsReading(machine: CacheSSM.M, addr: nat)
+  {
+    && machine.M?
+    && addr in machine.disk_idx_to_cache_idx
+    && machine.disk_idx_to_cache_idx[addr].Some?
+    && machine.disk_idx_to_cache_idx[addr].value in machine.entries
+    && machine.entries[machine.disk_idx_to_cache_idx[addr].value].Reading?
+  }
+
+  predicate IsWriting(machine: CacheSSM.M, addr: nat)
+  {
+    && machine.M?
+    && addr in machine.disk_idx_to_cache_idx
+    && machine.disk_idx_to_cache_idx[addr].Some?
+    && machine.disk_idx_to_cache_idx[addr].value in machine.statuses
+    && machine.statuses[machine.disk_idx_to_cache_idx[addr].value].Writeback?
+  }
+
+  predicate InverseMapConsistent(machine: CacheSSM.M, i: nat)
+  {
+    && machine.M?
+    && i in machine.disk_idx_to_cache_idx ==>
+      && machine.disk_idx_to_cache_idx[i].Some? ==>
+        && machine.disk_idx_to_cache_idx[i].value in machine.entries
+        && (machine.entries[machine.disk_idx_to_cache_idx[i].value].Reading?
+          || machine.entries[machine.disk_idx_to_cache_idx[i].value].Entry?)
+        && machine.entries[machine.disk_idx_to_cache_idx[i].value].disk_idx == i
+  }
+
+  predicate Inv(s: A.Variables) {
+    && s.machine.M?
+    && (forall i :: i in s.machine.statuses <==>
+        (i in s.machine.entries && s.machine.entries[i].Entry?))
+    && (forall i | i in s.machine.entries ::
+        (s.machine.entries[i].Entry? || s.machine.entries[i].Reading?) ==>
+            s.machine.entries[i].disk_idx in s.machine.disk_idx_to_cache_idx &&
+            s.machine.disk_idx_to_cache_idx[s.machine.entries[i].disk_idx] == Some(i))
+
+    && (forall i :: InverseMapConsistent(s.machine, i))
+
+    && s.disk.reqReads.Keys !! s.disk.respReads.Keys
+    && s.disk.reqWrites.Keys !! s.disk.respWrites.Keys
+
+    && s.machine.read_reqs !! s.machine.read_resps.Keys
+    && (forall rid1, rid2 | rid1 in s.disk.reqReads && rid2 in s.disk.reqReads && rid1 != rid2 ::
+          s.disk.reqReads[rid1].addr != s.disk.reqReads[rid2].addr)
+    && (forall rid1, rid2 | rid1 in s.disk.respReads && rid2 in s.disk.respReads && rid1 != rid2 ::
+          s.disk.respReads[rid1].addr != s.disk.respReads[rid2].addr)
+    && (forall rid1, rid2 | rid1 in s.disk.reqReads && rid2 in s.disk.respReads ::
+          s.disk.reqReads[rid1].addr != s.disk.respReads[rid2].addr)
+    && (forall rid1 | rid1 in s.disk.reqReads :: s.disk.reqReads[rid1].addr !in s.machine.read_reqs)
+    && (forall rid1 | rid1 in s.disk.reqReads :: s.disk.reqReads[rid1].addr !in s.machine.read_resps)
+    && (forall rid2 | rid2 in s.disk.respReads :: s.disk.respReads[rid2].addr !in s.machine.read_reqs)
+    && (forall rid2 | rid2 in s.disk.respReads :: s.disk.respReads[rid2].addr !in s.machine.read_resps)
+    && (forall rid1 | rid1 in s.disk.reqReads :: IsReading(s.machine, s.disk.reqReads[rid1].addr))
+    && (forall rid2 | rid2 in s.disk.respReads :: IsReading(s.machine, s.disk.respReads[rid2].addr))
+    && (forall addr | addr in s.machine.read_reqs :: IsReading(s.machine, addr))
+    && (forall addr | addr in s.machine.read_resps :: IsReading(s.machine, addr))
+
+    && s.machine.write_reqs.Keys !! s.machine.write_resps
+    && (forall rid1, rid2 | rid1 in s.disk.reqWrites && rid2 in s.disk.respWrites ::
+          s.disk.reqWrites[rid1].addr != s.disk.respWrites[rid2].addr)
+    && (forall rid1, rid2 | rid1 in s.disk.reqWrites && rid2 in s.disk.reqWrites && rid1 != rid2 ::
+          s.disk.reqWrites[rid1].addr != s.disk.reqWrites[rid2].addr)
+    && (forall rid1, rid2 | rid1 in s.disk.respWrites && rid2 in s.disk.respWrites && rid1 != rid2 ::
+          s.disk.respWrites[rid1].addr != s.disk.respWrites[rid2].addr)
+    && (forall rid1 | rid1 in s.disk.reqWrites :: s.disk.reqWrites[rid1].addr !in s.machine.write_reqs)
+    && (forall rid1 | rid1 in s.disk.reqWrites :: s.disk.reqWrites[rid1].addr !in s.machine.write_resps)
+    && (forall rid2 | rid2 in s.disk.respWrites :: s.disk.respWrites[rid2].addr !in s.machine.write_reqs)
+    && (forall rid2 | rid2 in s.disk.respWrites :: s.disk.respWrites[rid2].addr !in s.machine.write_resps)
+    && (forall rid1 | rid1 in s.disk.reqWrites :: IsWriting(s.machine, s.disk.reqWrites[rid1].addr))
+    && (forall rid2 | rid2 in s.disk.respWrites :: IsWriting(s.machine, s.disk.respWrites[rid2].addr))
+    && (forall addr | addr in s.machine.write_reqs :: IsWriting(s.machine, addr))
+    && (forall addr | addr in s.machine.write_resps :: IsWriting(s.machine, addr))
+
+    && s.machine.tickets.Keys !! s.machine.stubs.Keys
+  }
+
+  lemma InitImpliesInv(s: A.Variables)
+  requires A.Init(s)
+  ensures Inv(s)
+  {
+  }
+
+  lemma Start_PreservesInv(s: A.Variables, s': A.Variables, rid: RequestId, input: CacheIfc.Input)
+  requires Inv(s)
+  requires A.NewTicket(s, s', rid, input)
+  ensures Inv(s')
+  {
+    assume false;
+    assert s'.machine.entries == s.machine.entries;
+    assert s'.machine.statuses == s.machine.statuses;
+    assert s'.machine.read_reqs == s.machine.read_reqs;
+    assert s'.machine.read_resps == s.machine.read_resps;
+    assert s'.machine.write_reqs == s.machine.write_reqs;
+    assert s'.machine.write_resps == s.machine.write_resps;
+
+    assert forall i :: InverseMapConsistent(s.machine, i) ==> InverseMapConsistent(s'.machine, i);
+    assert forall i :: IsReading(s.machine, i) ==> IsReading(s'.machine, i);
+    assert forall i :: IsWriting(s.machine, i) ==> IsWriting(s'.machine, i);
+  }
+
+  lemma End_PreservesInv(s: A.Variables, s': A.Variables, rid: RequestId, output: CacheIfc.Output)
+  requires Inv(s)
+  requires A.ConsumeStub(s, s', rid, output)
+  ensures Inv(s')
+  {
+    assume false;
+    assert s'.machine.entries == s.machine.entries;
+    assert s'.machine.statuses == s.machine.statuses;
+
+    assert forall i :: InverseMapConsistent(s.machine, i) ==> InverseMapConsistent(s'.machine, i);
+    assert forall i :: IsReading(s.machine, i) ==> IsReading(s'.machine, i);
+    assert forall i :: IsWriting(s.machine, i) ==> IsWriting(s'.machine, i);
+  }
+
+  lemma StartRead_PreservesInv(s: A.Variables, s': A.Variables, cache_idx: nat, disk_idx: nat)
+  requires Inv(s)
+  requires CacheSSM.StartRead(s.machine, s'.machine, cache_idx, disk_idx)
+  requires s'.disk == s.disk
+  ensures Inv(s')
+  {
+    assert forall i :: InverseMapConsistent(s.machine, i) ==> InverseMapConsistent(s'.machine, i);
+    assert forall i :: IsReading(s.machine, i) ==> IsReading(s'.machine, i);
+    assert forall i :: IsWriting(s.machine, i) ==> IsWriting(s'.machine, i);
+  }
+
+  lemma FinishRead_PreservesInv(s: A.Variables, s': A.Variables, cache_idx: nat, disk_idx: nat)
+  requires Inv(s)
+  requires CacheSSM.FinishRead(s.machine, s'.machine, cache_idx, disk_idx)
+  requires s'.disk == s.disk
+  ensures Inv(s')
+  {
+    assert forall i :: InverseMapConsistent(s.machine, i) ==> InverseMapConsistent(s'.machine, i);
+    forall i | i != disk_idx && IsReading(s.machine, i)
+    ensures IsReading(s'.machine, i)
+    {
+      assert InverseMapConsistent(s.machine, i);
+    }
+    assert forall i :: IsWriting(s.machine, i) ==> IsWriting(s'.machine, i);
+  }
+
+  lemma StartWriteback_PreservesInv(s: A.Variables, s': A.Variables, cache_idx: nat)
+  requires Inv(s)
+  requires CacheSSM.StartWriteback(s.machine, s'.machine, cache_idx)
+  requires s'.disk == s.disk
+  ensures Inv(s')
+  {
+    assert forall i :: InverseMapConsistent(s.machine, i) ==> InverseMapConsistent(s'.machine, i);
+    assert forall i :: IsReading(s.machine, i) ==> IsReading(s'.machine, i);
+    assert forall i :: IsWriting(s.machine, i) ==> IsWriting(s'.machine, i);
+  }
+
+  lemma FinishWriteback_PreservesInv(s: A.Variables, s': A.Variables, cache_idx: nat)
+  requires Inv(s)
+  requires CacheSSM.FinishWriteback(s.machine, s'.machine, cache_idx)
+  requires s'.disk == s.disk
+  ensures Inv(s')
+  {
+    assert forall i :: InverseMapConsistent(s.machine, i) ==> InverseMapConsistent(s'.machine, i);
+    assert forall i :: IsReading(s.machine, i) ==> IsReading(s'.machine, i);
+    forall i | i != s.machine.entries[cache_idx].disk_idx && IsWriting(s.machine, i)
+    ensures IsWriting(s'.machine, i);
+    {
+      assert InverseMapConsistent(s.machine, i);
+    }
+  }
+
+  lemma Evict_PreservesInv(s: A.Variables, s': A.Variables, cache_idx: nat)
+  requires Inv(s)
+  requires CacheSSM.Evict(s.machine, s'.machine, cache_idx)
+  requires s'.disk == s.disk
+  ensures Inv(s')
+  {
+    assert forall i :: InverseMapConsistent(s.machine, i) ==> InverseMapConsistent(s'.machine, i);
+    assert forall i :: IsReading(s.machine, i) ==> IsReading(s'.machine, i);
+    assert forall i :: IsWriting(s.machine, i) ==> IsWriting(s'.machine, i);
+  }
+
+  lemma ObserveCleanForSync_PreservesInv(s: A.Variables, s': A.Variables, cache_idx: nat, rid: RequestId)
+  requires Inv(s)
+  requires CacheSSM.ObserveCleanForSync(s.machine, s'.machine, cache_idx, rid)
+  requires s'.disk == s.disk
+  ensures Inv(s')
+  {
+    assert forall i :: InverseMapConsistent(s.machine, i) ==> InverseMapConsistent(s'.machine, i);
+    assert forall i :: IsReading(s.machine, i) ==> IsReading(s'.machine, i);
+    assert forall i :: IsWriting(s.machine, i) ==> IsWriting(s'.machine, i);
+  }
+
+  lemma ApplyRead_PreservesInv(s: A.Variables, s': A.Variables, cache_idx: nat, rid: RequestId)
+  requires Inv(s)
+  requires CacheSSM.ApplyRead(s.machine, s'.machine, cache_idx, rid)
+  requires s'.disk == s.disk
+  ensures Inv(s')
+  {
+    assert forall i :: InverseMapConsistent(s.machine, i) ==> InverseMapConsistent(s'.machine, i);
+    assert forall i :: IsReading(s.machine, i) ==> IsReading(s'.machine, i);
+    assert forall i :: IsWriting(s.machine, i) ==> IsWriting(s'.machine, i);
+  }
+
+  lemma ApplyWrite_PreservesInv(s: A.Variables, s': A.Variables, cache_idx: nat, rid: RequestId)
+  requires Inv(s)
+  requires CacheSSM.ApplyWrite(s.machine, s'.machine, cache_idx, rid)
+  requires s'.disk == s.disk
+  ensures Inv(s')
+  {
+    assert forall i :: InverseMapConsistent(s.machine, i) ==> InverseMapConsistent(s'.machine, i);
+    assert forall i :: IsReading(s.machine, i) ==> IsReading(s'.machine, i);
+    assert forall i :: IsWriting(s.machine, i) ==> IsWriting(s'.machine, i);
+  }
+
+  lemma MarkDirty_PreservesInv(s: A.Variables, s': A.Variables, cache_idx: nat)
+  requires Inv(s)
+  requires CacheSSM.MarkDirty(s.machine, s'.machine, cache_idx)
+  requires s'.disk == s.disk
+  ensures Inv(s')
+  {
+    assert forall i :: InverseMapConsistent(s.machine, i) ==> InverseMapConsistent(s'.machine, i);
+    assert forall i :: IsReading(s.machine, i) ==> IsReading(s'.machine, i);
+    assert forall i :: IsWriting(s.machine, i) ==> IsWriting(s'.machine, i);
+  }
+
+  lemma StartRead_Monotonic(s: A.Variables, s': A.Variables, rest: CacheSSM.M,
+      cache_idx: nat, disk_idx: nat)
+  requires Inv(A.Variables(s.disk, CacheSSM.dot(s.machine, rest)))
+  requires CacheSSM.StartRead(s.machine, s'.machine, cache_idx, disk_idx)
+  ensures CacheSSM.Internal(CacheSSM.dot(s.machine, rest), CacheSSM.dot(s'.machine, rest))
+  {
+    /*assert disk_idx in s.machine.read_reqs ==> IsReading(s.machine, disk_idx);
+    var f := CacheSSM.dot(s.machine, rest);
+    var f' := CacheSSM.dot(s'.machine, rest);
+    assert f'.M?;
+    assert (f'.entries == f.entries[cache_idx := CacheSSM.Reading(disk_idx)]);
+    assert (f'.disk_idx_to_cache_idx == f.disk_idx_to_cache_idx[disk_idx := Some(cache_idx)]);
+    assert (f'.read_reqs == f.read_reqs + {disk_idx});*/
+    assert CacheSSM.StartRead(CacheSSM.dot(s.machine, rest), CacheSSM.dot(s'.machine, rest), cache_idx, disk_idx);
+    assert CacheSSM.InternalStep(CacheSSM.dot(s.machine, rest), CacheSSM.dot(s'.machine, rest), CacheSSM.StartReadStep(cache_idx, disk_idx));
+  }
+
+  lemma FinishRead_Monotonic(s: A.Variables, s': A.Variables, rest: CacheSSM.M,
+      cache_idx: nat, disk_idx: nat)
+  requires Inv(A.Variables(s.disk, CacheSSM.dot(s.machine, rest)))
+  requires CacheSSM.FinishRead(s.machine, s'.machine, cache_idx, disk_idx)
+  ensures CacheSSM.Internal(CacheSSM.dot(s.machine, rest), CacheSSM.dot(s'.machine, rest))
+  {
+    assert CacheSSM.InternalStep(CacheSSM.dot(s.machine, rest), CacheSSM.dot(s'.machine, rest), CacheSSM.FinishReadStep(cache_idx, disk_idx));
+  }
+
+  lemma StartWriteback_Monotonic(s: A.Variables, s': A.Variables, rest: CacheSSM.M,
+      cache_idx: nat)
+  requires Inv(A.Variables(s.disk, CacheSSM.dot(s.machine, rest)))
+  requires CacheSSM.StartWriteback(s.machine, s'.machine, cache_idx)
+  ensures CacheSSM.Internal(CacheSSM.dot(s.machine, rest), CacheSSM.dot(s'.machine, rest))
+  {
+    var disk_idx := s.machine.entries[cache_idx].disk_idx;
+    var f := CacheSSM.dot(s.machine, rest);
+    assert disk_idx in f.write_reqs ==> IsWriting(f, disk_idx);
+    assert CacheSSM.StartWriteback(CacheSSM.dot(s.machine, rest), CacheSSM.dot(s'.machine, rest), cache_idx);
+    assert CacheSSM.InternalStep(CacheSSM.dot(s.machine, rest), CacheSSM.dot(s'.machine, rest), CacheSSM.StartWritebackStep(cache_idx));
+  }
+
+  lemma FinishWriteback_Monotonic(s: A.Variables, s': A.Variables, rest: CacheSSM.M,
+      cache_idx: nat)
+  requires Inv(A.Variables(s.disk, CacheSSM.dot(s.machine, rest)))
+  requires CacheSSM.FinishWriteback(s.machine, s'.machine, cache_idx)
+  ensures CacheSSM.Internal(CacheSSM.dot(s.machine, rest), CacheSSM.dot(s'.machine, rest))
+  {
+    assert CacheSSM.InternalStep(CacheSSM.dot(s.machine, rest), CacheSSM.dot(s'.machine, rest), CacheSSM.FinishWritebackStep(cache_idx));
+  }
+
+  lemma Evict_Monotonic(s: A.Variables, s': A.Variables, rest: CacheSSM.M,
+      cache_idx: nat)
+  requires Inv(A.Variables(s.disk, CacheSSM.dot(s.machine, rest)))
+  requires CacheSSM.Evict(s.machine, s'.machine, cache_idx)
+  ensures CacheSSM.Internal(CacheSSM.dot(s.machine, rest), CacheSSM.dot(s'.machine, rest))
+  {
+    assert CacheSSM.InternalStep(CacheSSM.dot(s.machine, rest), CacheSSM.dot(s'.machine, rest), CacheSSM.EvictStep(cache_idx));
+  }
+
+  lemma ObserveCleanForSync_Monotonic(s: A.Variables, s': A.Variables, rest: CacheSSM.M,
+      cache_idx: nat, rid: RequestId)
+  requires Inv(A.Variables(s.disk, CacheSSM.dot(s.machine, rest)))
+  requires CacheSSM.ObserveCleanForSync(s.machine, s'.machine, cache_idx, rid)
+  ensures CacheSSM.Internal(CacheSSM.dot(s.machine, rest), CacheSSM.dot(s'.machine, rest))
+  {
+    assert CacheSSM.InternalStep(CacheSSM.dot(s.machine, rest), CacheSSM.dot(s'.machine, rest), CacheSSM.ObserveCleanForSyncStep(cache_idx, rid));
+  }
+
+  lemma ApplyRead_Monotonic(s: A.Variables, s': A.Variables, rest: CacheSSM.M,
+      cache_idx: nat, rid: RequestId)
+  requires Inv(A.Variables(s.disk, CacheSSM.dot(s.machine, rest)))
+  requires CacheSSM.ApplyRead(s.machine, s'.machine, cache_idx, rid)
+  ensures CacheSSM.Internal(CacheSSM.dot(s.machine, rest), CacheSSM.dot(s'.machine, rest))
+  {
+    assert CacheSSM.ApplyRead(CacheSSM.dot(s.machine, rest), CacheSSM.dot(s'.machine, rest), cache_idx, rid);
+    assert CacheSSM.InternalStep(CacheSSM.dot(s.machine, rest), CacheSSM.dot(s'.machine, rest), CacheSSM.ApplyReadStep(cache_idx, rid));
+  }
+
+  lemma ApplyWrite_Monotonic(s: A.Variables, s': A.Variables, rest: CacheSSM.M,
+      cache_idx: nat, rid: RequestId)
+  requires Inv(A.Variables(s.disk, CacheSSM.dot(s.machine, rest)))
+  requires CacheSSM.ApplyWrite(s.machine, s'.machine, cache_idx, rid)
+  ensures CacheSSM.Internal(CacheSSM.dot(s.machine, rest), CacheSSM.dot(s'.machine, rest))
+  {
+    assert CacheSSM.ApplyWrite(CacheSSM.dot(s.machine, rest), CacheSSM.dot(s'.machine, rest), cache_idx, rid);
+    assert CacheSSM.InternalStep(CacheSSM.dot(s.machine, rest), CacheSSM.dot(s'.machine, rest), CacheSSM.ApplyWriteStep(cache_idx, rid));
+  }
+
+  lemma MarkDirty_Monotonic(s: A.Variables, s': A.Variables, rest: CacheSSM.M,
+      cache_idx: nat)
+  requires Inv(A.Variables(s.disk, CacheSSM.dot(s.machine, rest)))
+  requires CacheSSM.MarkDirty(s.machine, s'.machine, cache_idx)
+  ensures CacheSSM.Internal(CacheSSM.dot(s.machine, rest), CacheSSM.dot(s'.machine, rest))
+  {
+    assert CacheSSM.MarkDirty(CacheSSM.dot(s.machine, rest), CacheSSM.dot(s'.machine, rest), cache_idx);
+    assert CacheSSM.InternalStep(CacheSSM.dot(s.machine, rest), CacheSSM.dot(s'.machine, rest), CacheSSM.MarkDirtyStep(cache_idx));
+  }
+
+  lemma InternalMonotonic(s: A.Variables, s': A.Variables, rest: CacheSSM.M)
+  requires Inv(A.Variables(s.disk, CacheSSM.dot(s.machine, rest)))
+  requires CacheSSM.Internal(s.machine, s'.machine)
+  ensures CacheSSM.Internal(CacheSSM.dot(s.machine, rest), CacheSSM.dot(s'.machine, rest))
+  {
+    var step :| CacheSSM.InternalStep(s.machine, s'.machine, step);
+    match step {
+      case StartReadStep(cache_idx, disk_idx) => {
+        StartRead_Monotonic(s, s', rest, cache_idx, disk_idx);
+      }
+
+      case FinishReadStep(cache_idx, disk_idx) => {
+        FinishRead_Monotonic(s, s', rest, cache_idx, disk_idx);
+      }
+
+      case StartWritebackStep(cache_idx) => {
+        StartWriteback_Monotonic(s, s', rest, cache_idx);
+      }
+
+      case FinishWritebackStep(cache_idx) => {
+        FinishWriteback_Monotonic(s, s', rest, cache_idx);
+      }
+
+      case EvictStep(cache_idx) => {
+        Evict_Monotonic(s, s', rest, cache_idx);
+      }
+
+      case ObserveCleanForSyncStep(cache_idx, rid) => {
+        ObserveCleanForSync_Monotonic(s, s', rest, cache_idx, rid);
+      }
+
+      case ApplyReadStep(cache_idx, rid) => {
+        ApplyRead_Monotonic(s, s', rest, cache_idx, rid);
+      }
+
+      case ApplyWriteStep(cache_idx, rid) => {
+        ApplyWrite_Monotonic(s, s', rest, cache_idx, rid);
+      }
+
+      case MarkDirtyStep(cache_idx) => {
+        MarkDirty_Monotonic(s, s', rest, cache_idx);
+      }
+    }
+  }
+
+  lemma Machine_Internal_PreservesInv(s: A.Variables, s': A.Variables)
+  requires Inv(s)
+  requires Internal(s.machine, s'.machine)
+  requires s.disk == s'.disk
+  ensures Inv(s')
+  {
+    var step :| CacheSSM.InternalStep(s.machine, s'.machine, step);
+    match step {
+      case StartReadStep(cache_idx, disk_idx) =>
+        StartRead_PreservesInv(s, s', cache_idx, disk_idx);
+
+      case FinishReadStep(cache_idx, disk_idx) => 
+        FinishRead_PreservesInv(s, s', cache_idx, disk_idx);
+
+      case StartWritebackStep(cache_idx) =>
+        StartWriteback_PreservesInv(s, s', cache_idx);
+
+      case FinishWritebackStep(cache_idx) =>
+        FinishWriteback_PreservesInv(s, s', cache_idx);
+
+      case EvictStep(cache_idx) =>
+        Evict_PreservesInv(s, s', cache_idx);
+
+      case ObserveCleanForSyncStep(cache_idx, rid) =>
+        ObserveCleanForSync_PreservesInv(s, s', cache_idx, rid);
+
+      case ApplyReadStep(cache_idx, rid) =>
+        ApplyRead_PreservesInv(s, s', cache_idx, rid);
+
+      case ApplyWriteStep(cache_idx, rid) =>
+        ApplyWrite_PreservesInv(s, s', cache_idx, rid);
+
+      case MarkDirtyStep(cache_idx) =>
+        MarkDirty_PreservesInv(s, s', cache_idx);
+    }
+  }
+
+  lemma ProcessRead_PreservesInv(s: A.Variables, s': A.Variables, id: RequestId)
+  requires Inv(s)
+  requires AsyncDisk.ProcessRead(s.disk, s'.disk, id)
+  requires s.machine == s'.machine
+  ensures Inv(s')
+  {
+  }
+
+  lemma ProcessWrite_PreservesInv(s: A.Variables, s': A.Variables, id: RequestId)
+  requires Inv(s)
+  requires AsyncDisk.ProcessWrite(s.disk, s'.disk, id)
+  requires s.machine == s'.machine
+  ensures Inv(s')
+  {
+  }
+
+  lemma HavocConflictingWrites_PreservesInv(s: A.Variables, s': A.Variables, id: RequestId, id':RequestId)
+  requires Inv(s)
+  requires AsyncDisk.HavocConflictingWrites(s.disk, s'.disk, id, id')
+  requires s.machine == s'.machine
+  ensures Inv(s')
+  {
+  }
+
+  lemma HavocConflictingWriteRead_PreservesInv(s: A.Variables, s': A.Variables, id: RequestId,id': RequestId)
+  requires Inv(s)
+  requires AsyncDisk.HavocConflictingWriteRead(s.disk, s'.disk, id, id')
+  requires s.machine == s'.machine
+  ensures Inv(s')
+  {
+  }
+
+  lemma DiskInternal_PreservesInv(s: A.Variables, s': A.Variables)
+  requires Inv(s)
+  requires A.DiskInternal(s, s')
+  ensures Inv(s')
+  {
+    var step :| AsyncDisk.NextInternalStep(s.disk, s'.disk, step);
+    match step {
+      case ProcessReadStep(id) => ProcessRead_PreservesInv(s, s', id);
+      case ProcessWriteStep(id) => ProcessWrite_PreservesInv(s, s', id);
+      case HavocConflictingWritesStep(id, id') => HavocConflictingWrites_PreservesInv(s, s', id, id');
+      case HavocConflictingWriteReadStep(id, id') => HavocConflictingWriteRead_PreservesInv(s, s', id, id');
+    }
+  }
+
+  lemma Interaction_ReqWrite_PreservesInv(s: A.Variables, s': A.Variables, dop: DiskIfc.DiskOp)
+  requires Inv(s)
+  requires AsyncDisk.RecvWrite(s.disk, s'.disk, dop)
+  requires s.machine == CacheSSM.dot(s'.machine, CacheSSM.DiskWriteReq(dop.reqWrite.addr, dop.reqWrite.data))
+  ensures Inv(s')
+  {
+    var x := CacheSSM.DiskWriteReq(dop.reqWrite.addr, dop.reqWrite.data);
+    assert s.machine == CacheSSM.dot(s'.machine, x);
+
+    assert s'.machine.M?;
+    assert s.machine.entries == s'.machine.entries;
+    assert s.machine.statuses == s'.machine.statuses;
+    assert s.machine.disk_idx_to_cache_idx == s'.machine.disk_idx_to_cache_idx;
+    assert s.machine.tickets == s'.machine.tickets;
+    assert s.machine.stubs == s'.machine.stubs;
+
+    assert forall i :: InverseMapConsistent(s.machine, i) ==> InverseMapConsistent(s'.machine, i);
+    assert forall i :: IsReading(s.machine, i) ==> IsReading(s'.machine, i);
+    assert forall i :: IsWriting(s.machine, i) ==> IsWriting(s'.machine, i);
+  }
+
+  lemma Interaction_RespWrite_PreservesInv(s: A.Variables, s': A.Variables, dop: DiskIfc.DiskOp)
+  requires Inv(s)
+  requires AsyncDisk.AckWrite(s.disk, s'.disk, dop)
+  requires s'.machine == CacheSSM.dot(s.machine, CacheSSM.DiskWriteResp(dop.respWrite.addr))
+  ensures Inv(s')
+  {
+    var x := CacheSSM.DiskWriteResp(dop.respWrite.addr);
+    assert s'.machine == CacheSSM.dot(s.machine, x);
+
+    assert s'.machine.M?;
+    assert s.machine.entries == s'.machine.entries;
+    assert s.machine.statuses == s'.machine.statuses;
+    assert s.machine.disk_idx_to_cache_idx == s'.machine.disk_idx_to_cache_idx;
+    assert s.machine.tickets == s'.machine.tickets;
+    assert s.machine.stubs == s'.machine.stubs;
+
+    assert forall i :: InverseMapConsistent(s.machine, i) ==> InverseMapConsistent(s'.machine, i);
+    assert forall i :: IsReading(s.machine, i) ==> IsReading(s'.machine, i);
+    assert forall i :: IsWriting(s.machine, i) ==> IsWriting(s'.machine, i);
+  }
+
+  lemma Interaction_ReqRead_PreservesInv(s: A.Variables, s': A.Variables, dop: DiskIfc.DiskOp)
+  requires Inv(s)
+  requires AsyncDisk.RecvRead(s.disk, s'.disk, dop)
+  requires s.machine == CacheSSM.dot(s'.machine, CacheSSM.DiskReadReq(dop.reqRead.addr))
+  ensures Inv(s')
+  {
+    /*assert s.machine.M?;
+    assert s'.machine.M? by {
+      if s'.machine == Fail {
+        assert CacheSSM.dot(Fail, CacheSSM.DiskReadReq(dop.reqRead.addr)) == Fail;
+        assert CacheSSM.dot(s'.machine, CacheSSM.DiskReadReq(dop.reqRead.addr)) == Fail;
+        assert s.machine == Fail;
+      }
+    }*/
+
+    var x := CacheSSM.DiskReadReq(dop.reqRead.addr);
+    assert s.machine == CacheSSM.dot(s'.machine, x);
+
+    assert s'.machine.M?;
+    assert s.machine.entries == s'.machine.entries;
+    assert s.machine.statuses == s'.machine.statuses;
+    assert s.machine.disk_idx_to_cache_idx == s'.machine.disk_idx_to_cache_idx;
+    assert s.machine.tickets == s'.machine.tickets;
+    assert s.machine.stubs == s'.machine.stubs;
+
+    assert forall i :: InverseMapConsistent(s.machine, i) ==> InverseMapConsistent(s'.machine, i);
+    assert forall i :: IsReading(s.machine, i) ==> IsReading(s'.machine, i);
+    assert forall i :: IsWriting(s.machine, i) ==> IsWriting(s'.machine, i);
+  }
+
+  lemma Interaction_RespRead_PreservesInv(s: A.Variables, s': A.Variables, dop: DiskIfc.DiskOp)
+  requires Inv(s)
+  requires AsyncDisk.AckRead(s.disk, s'.disk, dop)
+  requires s'.machine == CacheSSM.dot(s.machine, CacheSSM.DiskReadResp(dop.respRead.addr, dop.respRead.data))
+  ensures Inv(s')
+  {
+    var x := CacheSSM.DiskReadResp(dop.respRead.addr, dop.respRead.data);
+    assert s'.machine == CacheSSM.dot(s.machine, x);
+
+    assert s'.machine.M?;
+    assert s.machine.entries == s'.machine.entries;
+    assert s.machine.statuses == s'.machine.statuses;
+    assert s.machine.disk_idx_to_cache_idx == s'.machine.disk_idx_to_cache_idx;
+    assert s.machine.tickets == s'.machine.tickets;
+    assert s.machine.stubs == s'.machine.stubs;
+
+    assert forall i :: InverseMapConsistent(s.machine, i) ==> InverseMapConsistent(s'.machine, i);
+    assert forall i :: IsReading(s.machine, i) ==> IsReading(s'.machine, i);
+    assert forall i :: IsWriting(s.machine, i) ==> IsWriting(s'.machine, i);
+  }
+
+  lemma Interaction_PreservesInv(s: A.Variables, s': A.Variables, dop: DiskIfc.DiskOp)
+  requires Inv(s)
+  requires A.Interaction(s, s', dop)
+  ensures Inv(s')
+  {
+    match dop {
+      case ReqReadOp(id, reqRead) => {
+        Interaction_ReqRead_PreservesInv(s, s', dop);
+      }
+      case ReqWriteOp(id, reqWrite) => {
+        Interaction_ReqWrite_PreservesInv(s, s', dop);
+      }
+      case RespReadOp(id, respRead) => {
+        Interaction_RespRead_PreservesInv(s, s', dop);
+      }
+      case RespWriteOp(id, respWrite) => {
+        Interaction_RespWrite_PreservesInv(s, s', dop);
+      }
+    }
+  }
+
+  lemma Internal_PreservesInv(s: A.Variables, s': A.Variables)
+  requires Inv(s)
+  requires A.Internal(s, s')
+  ensures Inv(s')
+  {
+    var step :| A.InternalStep(s, s', step);
+    match step {
+      case MachineStep(shard, shard', rest) => {
+        InternalMonotonic(
+            A.Variables(s.disk, shard),
+            A.Variables(s.disk, shard'),
+            rest);
+        Machine_Internal_PreservesInv(s, s');
+      }
+      case InteractionStep(dop) => {
+        Interaction_PreservesInv(s, s', dop);
+      }
+      case DiskInternalStep => {
+        DiskInternal_PreservesInv(s, s');
+      }
+    }
+  }
+
+  lemma NextPreservesInv(s: A.Variables, s': A.Variables, op: ifc.Op)
+  requires Inv(s)
+  requires A.Next(s, s', op)
+  ensures Inv(s')
+  {
+    match op {
+      case Start(rid, input) => {
+        Start_PreservesInv(s, s', rid, input);
+      }
+      case End(rid, output) => {
+        End_PreservesInv(s, s', rid, output);
+      }
+      case CrashOp => {
+        InitImpliesInv(s');
+      }
+      case InternalOp => {
+        Internal_PreservesInv(s, s');
+      }
+    }
+  }
+}
